Set_Graphs/Graph_Algorithms/BFS_Subprocedures.thy
@@ -39,26 +39,26 @@ proof(goal_cases)
   have a: "vset_inv vs \<Longrightarrow>
        \<forall>v vset. lookup G v = Some vset \<longrightarrow> vset_inv vset \<Longrightarrow>
        lookup G u = Some x2 \<Longrightarrow>
-       b \<in> [case if a = u then Some (x2 \<union>\<^sub>G vs) else lookup G a of None \<Rightarrow> \<emptyset>\<^sub>N | Some vset \<Rightarrow> vset]\<^sub>s \<Longrightarrow>
+       b \<in> [case if a = u then Some (x2 \<union>\<^sub>G vs) else lookup G a of None \<Rightarrow> \<emptyset>\<^sub>V | Some vset \<Rightarrow> vset]\<^sub>s \<Longrightarrow>
        b \<notin> [vs]\<^sub>s \<Longrightarrow> lookup G a = Some x2a \<Longrightarrow> b \<in> [x2a]\<^sub>s" for a b x2 x2a
     by (auto intro: case_split[of "a = u"] simp add: set_ops.set_union)
   have b: "\<forall>v vset. lookup G v = Some vset \<longrightarrow> vset_inv vset \<Longrightarrow>
        lookup G u = Some x2 \<Longrightarrow>
-       b \<in> [case if a = u then Some (x2 \<union>\<^sub>G vs) else lookup G a of None \<Rightarrow> \<emptyset>\<^sub>N | Some vset \<Rightarrow> vset]\<^sub>s \<Longrightarrow>
+       b \<in> [case if a = u then Some (x2 \<union>\<^sub>G vs) else lookup G a of None \<Rightarrow> \<emptyset>\<^sub>V | Some vset \<Rightarrow> vset]\<^sub>s \<Longrightarrow>
        b \<notin> [vs]\<^sub>s \<Longrightarrow> \<exists>y. lookup G a = Some y" for a b x2 x2a 
     using Graph.vset.emptyD(1) domIff by (fastforce intro: case_split[of "a = u"])
-  have c: "b \<in> [case if a = u then Some vs else lookup G a of None \<Rightarrow> \<emptyset>\<^sub>N | Some vset \<Rightarrow> vset]\<^sub>s \<Longrightarrow>
+  have c: "b \<in> [case if a = u then Some vs else lookup G a of None \<Rightarrow> \<emptyset>\<^sub>V | Some vset \<Rightarrow> vset]\<^sub>s \<Longrightarrow>
        b \<notin> [vs]\<^sub>s \<Longrightarrow> lookup G a = Some x2 \<Longrightarrow> b \<in> [x2]\<^sub>s" for a b x2
      by (fastforce intro: case_split[of "a = u"])
   have d: "\<forall>v vset. lookup G v = Some vset \<longrightarrow> vset_inv vset \<Longrightarrow>
-           b \<in> [case if a = u then Some vs else lookup G a of None \<Rightarrow> \<emptyset>\<^sub>N | Some vset \<Rightarrow> vset]\<^sub>s \<Longrightarrow>
+           b \<in> [case if a = u then Some vs else lookup G a of None \<Rightarrow> \<emptyset>\<^sub>V | Some vset \<Rightarrow> vset]\<^sub>s \<Longrightarrow>
            b \<notin> [vs]\<^sub>s \<Longrightarrow> \<exists>y. lookup G a = Some y" for a b 
     using Graph.vset.emptyD(3) domIff by (fastforce intro: case_split[of "a = u"])
   show ?case 
     using 1  Graph.vset.set.set_empty 
     by(auto split: if_split option.split 
             simp add:  add_neighbs_def Graph.digraph_abs_def 
-                      Graph.neighbourhood_def Graph.adjmap.map_update Graph.graph_inv_def
+                      Graph.neighb_def Graph.adjmap.map_update Graph.graph_inv_def
                       Graph.vset.emptyD(3) Graph.vset.set.invar_empty
                       Graph.vset.set.set_isin set_ops.invar_union set_ops.set_union)
       (insert Graph.vset.emptyD(3), auto intro: a b c d)   
@@ -81,12 +81,12 @@ assumes fold_adjmap:"\<And> N f acc. vset_inv N \<Longrightarrow> \<exists> xs. 
 
 begin
 
-abbreviation "neighbourhood' \<equiv> Graph.neighbourhood G" 
-notation "neighbourhood'" ("\<N>\<^sub>G _" 100)
+abbreviation "neighb' \<equiv> Graph.neighb G" 
+notation "neighb'" ("\<N>\<^sub>G _" 100)
 
 definition next_frontier::"'vset \<Rightarrow> 'vset \<Rightarrow> 'vset"  where
 "next_frontier frontier vis= 
-   fold_vset (\<lambda> u nf. nf \<union>\<^sub>G ((\<N>\<^sub>G u) -\<^sub>G vis)) frontier \<emptyset>\<^sub>N"
+   fold_vset (\<lambda> u nf. nf \<union>\<^sub>G ((\<N>\<^sub>G u) -\<^sub>G vis)) frontier \<emptyset>\<^sub>V"
 declare Graph.vset.set.set_empty[simp] Graph.vset.set.set_isin[simp] Graph.vset.set.set_insert[simp]
         Graph.vset.set.set_delete[simp] Graph.vset.set.invar_empty[simp] 
         Graph.vset.set.invar_insert[simp] Graph.vset.set.invar_delete[simp]
@@ -101,7 +101,7 @@ lemma next_frontier:
          (\<Union> {Pair_Graph.neighbourhood (Graph.digraph_abs G) u | u . u \<in> t_set frontier}) - t_set vis"
 proof-
   assume assms: "vset_inv frontier" "vset_inv vis" "Graph.graph_inv G"
-  have goal1_gen:"vset_inv (foldr (\<lambda>u nf. nf \<union>\<^sub>G (\<N>\<^sub>G u -\<^sub>G vis)) xs \<emptyset>\<^sub>N)" for xs
+  have goal1_gen:"vset_inv (foldr (\<lambda>u nf. nf \<union>\<^sub>G (\<N>\<^sub>G u -\<^sub>G vis)) xs \<emptyset>\<^sub>V)" for xs
    using assms 
     by (induction xs)(auto split: option.split)
 
@@ -111,34 +111,34 @@ proof-
   hence "foldr (\<lambda>u nf. nf \<union> [(\<N>\<^sub>G u -\<^sub>G vis)]\<^sub>s) xs {} =
                    foldr (\<lambda>u nf. nf \<union> [(\<N>\<^sub>G u -\<^sub>G vis)]\<^sub>s) (remdups xs) {}" for xs
     by(induction xs) auto
-  moreover have "foldr (\<lambda>u nf. nf \<union> [(\<N>\<^sub>G u -\<^sub>G vis)]\<^sub>s) xs {} = [(foldr (\<lambda>u nf. nf \<union>\<^sub>G (\<N>\<^sub>G u -\<^sub>G vis)) xs \<emptyset>\<^sub>N)]\<^sub>s"  for xs
+  moreover have "foldr (\<lambda>u nf. nf \<union> [(\<N>\<^sub>G u -\<^sub>G vis)]\<^sub>s) xs {} = [(foldr (\<lambda>u nf. nf \<union>\<^sub>G (\<N>\<^sub>G u -\<^sub>G vis)) xs \<emptyset>\<^sub>V)]\<^sub>s"  for xs
     by (induction xs)
        (simp add: assms(2) assms(3) goal1_gen)+
-  ultimately have "[(foldr (\<lambda>u nf. nf \<union>\<^sub>G (\<N>\<^sub>G u -\<^sub>G vis)) xs \<emptyset>\<^sub>N)]\<^sub>s =
-                      [(foldr (\<lambda>u nf. nf \<union>\<^sub>G (\<N>\<^sub>G u -\<^sub>G vis)) (remdups xs) \<emptyset>\<^sub>N)]\<^sub>s" for xs
+  ultimately have "[(foldr (\<lambda>u nf. nf \<union>\<^sub>G (\<N>\<^sub>G u -\<^sub>G vis)) xs \<emptyset>\<^sub>V)]\<^sub>s =
+                      [(foldr (\<lambda>u nf. nf \<union>\<^sub>G (\<N>\<^sub>G u -\<^sub>G vis)) (remdups xs) \<emptyset>\<^sub>V)]\<^sub>s" for xs
     by auto
   moreover obtain xs where xs_props:
        "set xs = [frontier]\<^sub>s"
        "[next_frontier frontier vis]\<^sub>s =
-          [foldr (\<lambda>u nf. nf \<union>\<^sub>G (\<N>\<^sub>G u -\<^sub>G vis)) xs \<emptyset>\<^sub>N]\<^sub>s"
+          [foldr (\<lambda>u nf. nf \<union>\<^sub>G (\<N>\<^sub>G u -\<^sub>G vis)) xs \<emptyset>\<^sub>V]\<^sub>s"
     using fold_vset[OF assms(1)]
     by(auto simp add: next_frontier_def) metis  
   ultimately obtain xs' where xs'_props: 
        "set xs' = [frontier]\<^sub>s"
        "[next_frontier frontier vis]\<^sub>s =
-           [foldr (\<lambda>u nf. nf \<union>\<^sub>G (\<N>\<^sub>G u -\<^sub>G vis)) xs' \<emptyset>\<^sub>N]\<^sub>s"
+           [foldr (\<lambda>u nf. nf \<union>\<^sub>G (\<N>\<^sub>G u -\<^sub>G vis)) xs' \<emptyset>\<^sub>V]\<^sub>s"
        "distinct xs'"
     using distinct_remdups set_remdups
     by (metis )
-  moreover have "[foldr (\<lambda>u nf. nf \<union>\<^sub>G (\<N>\<^sub>G u -\<^sub>G vis)) xs' \<emptyset>\<^sub>N]\<^sub>s =
-                    \<Union> {neighbourhood [G]\<^sub>g u |u. u \<in> set xs'} - [vis]\<^sub>s"
+  moreover have "[foldr (\<lambda>u nf. nf \<union>\<^sub>G (\<N>\<^sub>G u -\<^sub>G vis)) xs' \<emptyset>\<^sub>V]\<^sub>s =
+                    \<Union> {neighbourhood [G]\<^sub>G u |u. u \<in> set xs'} - [vis]\<^sub>s"
     by(induction xs')
       (auto simp add: Graph.vset.emptyD(1) assms(2) assms(3) goal1_gen)+
 
-  ultimately show "[next_frontier frontier vis]\<^sub>s = \<Union> {neighbourhood [G]\<^sub>g u |u. u \<in> [frontier]\<^sub>s} - [vis]\<^sub>s"
+  ultimately show "[next_frontier frontier vis]\<^sub>s = \<Union> {neighbourhood [G]\<^sub>G u |u. u \<in> [frontier]\<^sub>s} - [vis]\<^sub>s"
     by presburger
 
-  have "vset_inv (foldr (\<lambda>u nf. nf \<union>\<^sub>G (\<N>\<^sub>G u -\<^sub>G vis)) xs \<emptyset>\<^sub>N)" for xs
+  have "vset_inv (foldr (\<lambda>u nf. nf \<union>\<^sub>G (\<N>\<^sub>G u -\<^sub>G vis)) xs \<emptyset>\<^sub>V)" for xs
    using assms 
     by (induction xs)(auto split: option.split intro!: Cons)
 
@@ -151,7 +151,7 @@ qed
 definition expand_tree::"'adjmap \<Rightarrow> 'vset \<Rightarrow> 'vset \<Rightarrow> 'adjmap" where
 "expand_tree BFS_tree frontier vis = 
    fold_adjmap 
-     (\<lambda> u nf. add_neighbs nf u (diff (neighbourhood' u) vis)) frontier BFS_tree"
+     (\<lambda> u nf. add_neighbs nf u (diff (\<N>\<^sub>G u) vis)) frontier BFS_tree"
 
 lemma expand_tree:
      "\<lbrakk>Graph.graph_inv BFS_tree; vset_inv frontier; vset_inv vis; Graph.graph_inv G\<rbrakk> \<Longrightarrow> 
@@ -165,10 +165,10 @@ lemma expand_tree:
 proof-
   assume assms: "Graph.graph_inv BFS_tree" "vset_inv frontier" "vset_inv vis" "Graph.graph_inv G"
   obtain xs where xs_prop:
-    "set xs = [frontier]\<^sub>s" "expand_tree BFS_tree frontier vis = foldr (\<lambda> u nf. add_neighbs nf u (diff (neighbourhood' u) vis)) xs BFS_tree"
+    "set xs = [frontier]\<^sub>s" "expand_tree BFS_tree frontier vis = foldr (\<lambda> u nf. add_neighbs nf u (diff (\<N>\<^sub>G u) vis)) xs BFS_tree"
     using fold_adjmap[OF assms(2), of _ BFS_tree]
     by (auto simp add: expand_tree_def)
-  have goal1_general:"Graph.graph_inv (foldr  (\<lambda> u nf. add_neighbs nf u (diff (neighbourhood' u) vis))
+  have goal1_general:"Graph.graph_inv (foldr  (\<lambda> u nf. add_neighbs nf u (diff (\<N>\<^sub>G u) vis))
                           xs BFS_tree)" for xs
   proof(induction xs)
     case Nil
@@ -181,11 +181,11 @@ proof-
   thus " Graph.graph_inv (expand_tree BFS_tree frontier vis)"
     by (simp add: xs_prop(2))
   have one_it_graph_abs:"Graph.graph_inv T \<Longrightarrow> 
-                 [(\<lambda> u nf. add_neighbs nf u (diff (neighbourhood' u) vis)) u T]\<^sub>g 
-               = [T]\<^sub>g \<union> {(u, v) |v. v \<in> neighbourhood [G]\<^sub>g u - [vis]\<^sub>s}" for u T
+                 [(\<lambda> u nf. add_neighbs nf u (diff (\<N>\<^sub>G u) vis)) u T]\<^sub>G 
+               = [T]\<^sub>G \<union> {(u, v) |v. v \<in> neighbourhood [G]\<^sub>G u - [vis]\<^sub>s}" for u T
     by(auto simp add: assms(3) assms(4) add_neighbs_digraph_abs)
 
-  have "[foldr (\<lambda> u nf. add_neighbs nf u (diff (neighbourhood' u) vis)) xs BFS_tree]\<^sub>g = [BFS_tree]\<^sub>g \<union> {(u, v) |u v. u \<in> [frontier]\<^sub>s \<and> v \<in> neighbourhood [G]\<^sub>g u - [vis]\<^sub>s}"
+  have "[foldr (\<lambda> u nf. add_neighbs nf u (diff (\<N>\<^sub>G u) vis)) xs BFS_tree]\<^sub>G = [BFS_tree]\<^sub>G \<union> {(u, v) |u v. u \<in> [frontier]\<^sub>s \<and> v \<in> neighbourhood [G]\<^sub>G u - [vis]\<^sub>s}"
     using xs_prop(1) assms(2)
   proof(induction xs arbitrary: frontier)
     case Nil
@@ -195,8 +195,8 @@ proof-
     show ?case 
     proof(cases "a \<in> set xs")
       case True
-      have heper: "[foldr (\<lambda> u nf. add_neighbs nf u (diff (neighbourhood' u) vis)) xs BFS_tree]\<^sub>g \<union> {(a, v) |v. v \<in> neighbourhood [G]\<^sub>g a - [vis]\<^sub>s} =
-    [BFS_tree]\<^sub>g \<union> {(u, v). u \<in> [frontier]\<^sub>s \<and> v \<in> neighbourhood [G]\<^sub>g u \<and> v \<notin> [vis]\<^sub>s}"
+      have heper: "[foldr (\<lambda> u nf. add_neighbs nf u (diff (\<N>\<^sub>G u) vis)) xs BFS_tree]\<^sub>G \<union> {(a, v) |v. v \<in> neighbourhood [G]\<^sub>G a - [vis]\<^sub>s} =
+    [BFS_tree]\<^sub>G \<union> {(u, v). u \<in> [frontier]\<^sub>s \<and> v \<in> neighbourhood [G]\<^sub>G u \<and> v \<notin> [vis]\<^sub>s}"
       using Cons.prems(1) True 
       by (subst Cons(1)[of frontier])(auto simp add: Cons.prems(2))
      show ?thesis 
@@ -211,8 +211,8 @@ proof-
      by(auto simp add: one_it_graph_abs goal1_general Cons(1)[of "vset_delete a frontier"] Cons.prems(2) Graph.vset.set.invar_delete del_set sym[OF Cons(2)])
  qed
 qed
-  thus "[expand_tree BFS_tree frontier vis]\<^sub>g =
-    [BFS_tree]\<^sub>g \<union> {(u, v) |u v. u \<in> [frontier]\<^sub>s \<and> v \<in> neighbourhood [G]\<^sub>g u - [vis]\<^sub>s}"
+  thus "[expand_tree BFS_tree frontier vis]\<^sub>G =
+    [BFS_tree]\<^sub>G \<union> {(u, v) |u v. u \<in> [frontier]\<^sub>s \<and> v \<in> neighbourhood [G]\<^sub>G u - [vis]\<^sub>s}"
     using xs_prop(2) by argo
 qed
 end
